# Problem

$$ B = \left(\frac{\sqrt{5} + 1}{1 + \sqrt{5} + \sqrt{3}} + \frac{\sqrt{5} - 1}{1 + \sqrt{3} - \sqrt{5}}\right)\left(\sqrt{3} - 4\sqrt{\frac{1}{3}} + 2\right) \cdot \sqrt{0.2} $$

> Solution

$$ B = \left(\frac{\sqrt{5} + 1}{1 + \sqrt{5} + \sqrt{3}} + \frac{\sqrt{5} - 1}{1 + \sqrt{3} - \sqrt{5}}\right)\left(\sqrt{3} - 4\left(\sqrt{\frac{1}{3}}\right) + 2\right) \cdot \sqrt{\frac{1}{5}} $$

$$ B = \left(\frac{\sqrt{5} + \sqrt{15} - 5 + 1 + \sqrt{3} - \sqrt{5} + \sqrt{5} + 5 + \sqrt{15} - 1 - \sqrt{5} - \sqrt{3}}{(1 + \sqrt{3})^2 - 5}\right) \left(\sqrt{3}- 4\left(\sqrt{\frac{1}{3}}\right) + 2\right)\cdot \sqrt{\frac{1}{5}} $$

$$ B = \left(\frac{2\sqrt{15}}{2\sqrt{3} - 1}\right)\left(\sqrt{3}- 4\left(\sqrt{\frac{1}{3}}\right) + 2\right)\cdot \sqrt{\frac{1}{5}} $$

$$ B = \left(\frac{2\sqrt{15}}{2\sqrt{3} - 1}\right)\left(\sqrt{3} - 4\left(\frac{1}{\sqrt{3}}\right ) + 2\right)\cdot\left(\frac{1}{\sqrt{5}}\right) $$

$$ B = \left(\frac{2\sqrt{15}}{2\sqrt{3} - 1}\right) \left(\frac{3 - 4 + 2\sqrt{3}}{\sqrt{3}}\right)\cdot\left(\frac{1}{\sqrt{5}}\right) $$

$$ B = \left(\frac{2\sqrt{15}}{2\sqrt{3} - 1}\right) \left(\frac{2\sqrt{3} - 1}{\sqrt{3}}\right)\cdot\left(\frac{1}{\sqrt{5}}\right)$$

$$ B = \left(\frac{2\sqrt{15}}{2\sqrt{3} - 1}\right) \left(\frac{2\sqrt{3} - 1}{\sqrt{15}}\right) $$

$$ B = \frac{2\sqrt{15}}{\sqrt{15}} $$

$$ B = 2 $$
